nrjgwrgöj

Games/gameLib_fix/Conditioning_Symm.lean
@@ -40,44 +40,28 @@ lemma Symm_Game_World.world_after_fst_transition {α β : Type u} (g : Symm_Game
 
 
 
+-- # Carelessness
+
+def careless
+  (f_law s_law : α → List β → (β → Prop)) (ini : α)
+  (obj : α → List β → γ) (swap : α → List β → β → α): Prop :=
+  ∀ ini : α , ∀ hist : List β, ∀ prehist : List β, (h : prehist ≠ []) → Hist_legal ini f_law s_law prehist →
+    obj ini (hist ++ prehist) = obj (swap ini prehist.tail (prehist.head h)) hist
 
 
-
-
-
-#exit
-
-
--- # Easy termination
-
-
-inductive Symm_Game_World.has_WL (g : Symm_Game_World α β) : Prop where
-| wf : g.is_fst_win → g.has_WL
-| ws : g.is_snd_win → g.has_WL
-
-
--- lemma Symm_Game_World.has_WL_init_end
---   (g : Symm_Game_World α β)
---   (hg : g.playable)
---   (P : Prop)
---   (hp : P)
---   (h : (P ∧ (¬ g.win_states g.init_game_state)) → g.has_WL) :
---   g.has_WL :=
---   by
---   obtain ⟨fs,ss,_,_⟩ := g.playable_has_strat hg
---   by_cases q2 : g.win_states g.init_game_state
---   · apply Symm_Game_World.has_WL.ws
---     use fs
---     intro _ _ _
---     use 0
---     constructor
---     · decide
---     · constructor
---       · apply q2
---       · intro t no
---         contradiction
---   · exact h ⟨hp, q2⟩
-
+lemma careless_singleton
+  (f_law s_law : α → List β → (β → Prop)) (ini : α)
+  (obj : α → List β → γ) (swap : α → List β → β → α) (hc : careless f_law s_law ini obj swap) :
+  ∀ ini : α , ∀ hist : List β, ∀ act : β, f_law ini [] act → obj ini (hist ++ [act]) = obj (swap ini [] (act)) hist
+  :=
+  by
+  intro ini hist act q
+  apply hc ini hist [act]
+  · apply List.noConfusion
+  · apply Hist_legal.cons
+    · rw [if_pos (by dsimp ; decide)]
+      exact q
+    · apply Hist_legal.nil
 
 
 
@@ -94,15 +78,13 @@ structure zSymm_Game_World (α β : Type _) extends Symm_Game_World α β where
 
 structure zSymm_Game (α β : Type _) extends zSymm_Game_World α β where
   /-- The first players strategy-/
-  fst_strat : Strategy α β
+  fst_strat : fStrategy tozSymm_Game_World.toSymm_Game_World.init_game_state tozSymm_Game_World.toSymm_Game_World.law tozSymm_Game_World.toSymm_Game_World.law
   /-- The second players strategy-/
-  snd_strat : Strategy α β
-  /-- The first players strategy is legal wrt. `law` and the second strategy-/
-  fst_lawful : Strategy_legal_fst init_game_state law fst_strat snd_strat
-  /-- The second players strategy is legal wrt. `law` and the first strategy-/
-  snd_lawful : Strategy_legal_snd init_game_state law fst_strat snd_strat
+  snd_strat : sStrategy tozSymm_Game_World.toSymm_Game_World.init_game_state tozSymm_Game_World.toSymm_Game_World.law tozSymm_Game_World.toSymm_Game_World.law
 
 
+
+-- # Deconditioned strats
 
 instance (l : List α): Decidable (l = []) :=
   by
@@ -110,14 +92,45 @@ instance (l : List α): Decidable (l = []) :=
   | [] => apply isTrue ; rfl
   | x :: L => apply isFalse ; exact List.cons_ne_nil x L
 
+lemma histDropLast_help (hist : List β) (q : hist ≠ []) : hist.dropLast.length + 1 = hist.length := by
+  rw [List.length_dropLast, Nat.sub_add_cancel]
+  rw [Nat.succ_le, List.length_pos]
+  exact q
+
+lemma Symm_Game_World.Hist_dropLast_legal (g : Symm_Game_World α β)
+  (lc : careless g.law g.law g.init_game_state g.law g.transition)
+  (f_act : β) (f_act_leg : g.law g.init_game_state [] f_act) (hist : List β)
+  (h : Hist_legal g.init_game_state g.law g.law hist) :
+  Hist_legal (g.world_after_fst f_act).init_game_state g.law g.law hist.dropLast := by
+  induction' hist with x l ih
+  · dsimp
+    apply Hist_legal.nil
+  · cases' h
+    rename_i sofar now
+    by_cases q : l ≠ []
+    · rw [List.dropLast_cons_of_ne_nil q]
+      apply Hist_legal.cons _ _ _ (ih sofar)
+      split_ifs with T
+      · rw [histDropLast_help _ q, Turn_fst_not_step] at T
+        rw [if_neg T] at now
+        rw [← List.dropLast_append_getLast q] at now
+        -- rw lc at now, but show that gestLast singleton is legal due to ih and Hist_legal_suffix
 
 
-def fst_strat_deconditioned (s_strat : Strategy α β) (f_act : β) (g : Symm_Game_World α β) : Strategy α β :=
-  (fun _ hist => if hist = [] then f_act else s_strat (g.world_after_fst f_act).init_game_state (hist.dropLast))
 
-def snd_strat_deconditioned (f_strat : Strategy α β) (f_act : β) (g : Symm_Game_World α β) : Strategy α β :=
+#check List.dropLast_cons_of_ne_nil
+
+#exit
+
+def Symm_Game_World.fst_strat_deconditioned (g : Symm_Game_World α β) (f_act : β) (f_act_leg : g.law g.init_game_state [] f_act)
+  (s_strat : sStrategy (g.world_after_fst f_act).init_game_state g.law g.law) : fStrategy g.init_game_state g.law g.law :=
+  (fun hist T leg => if q : hist = [] then ⟨f_act, (by rw [q]; exact f_act_leg)⟩ else s_strat (hist.dropLast) (by rw [histDropLast_help _ q, Turn_snd_fst_step] ; exact T) ())
+
+def Symm_Game_World.snd_strat_deconditioned (g : Symm_Game_World α β) (f_strat : Strategy α β) (f_act : β) (g : Symm_Game_World α β) : Strategy α β :=
   (fun _ hist => f_strat (g.world_after_fst f_act).init_game_state (hist.dropLast))
 
+
+#exit
 
 lemma Symm_Game_World.History_of_deconditioned
   (g: Symm_Game_World α β)
@@ -157,13 +170,147 @@ lemma Symm_Game_World.History_of_deconditioned
       rw [List.dropLast_concat]
 
 
+
+lemma Symm_Game_World.State_of_deconditioned
+  (g: Symm_Game_World α β)
+  (tb : g.transition_blind)
+  (fst_act: β)
+  (fst_act_legal: g.law g.init_game_state [] fst_act)
+  (f_strat s_strat : Strategy α β)
+  (turn : ℕ):
+  let fst_strat := fst_strat_deconditioned s_strat fst_act g
+  let snd_strat := snd_strat_deconditioned f_strat fst_act g
+  g.state_on_turn fst_strat snd_strat (turn + 1) =
+  (g.world_after_fst fst_act).state_on_turn f_strat s_strat turn :=
+  by
+  intro fst_strat snd_strat
+  cases' turn with t
+  · dsimp [state_on_turn]
+    rw [if_pos (by decide)]
+    dsimp [history_on_turn, History_on_turn]
+    rw [fst_strat_deconditioned, if_pos (by rfl)]
+  · dsimp [state_on_turn]
+    by_cases q : Turn_fst (t + 1)
+    · rw [if_pos q]
+      rw [Turn_fst_not_step] at q
+      rw [if_neg q]
+      dsimp [history_on_turn]
+      have := g.History_of_deconditioned fst_act f_strat s_strat t
+      dsimp at this
+      rw [this]
+      rw [snd_strat_deconditioned, List.dropLast_concat]
+      rw [← this]
+      clear this
+      have := tb.2 f_strat s_strat fst_act fst_act_legal
+      dsimp at this
+      specialize this t (f_strat (world_after_fst g fst_act).init_game_state (History_on_turn (world_after_fst g fst_act).init_game_state f_strat s_strat t))
+      rw [← Symm_Game_World.world_after_fst_init]
+      rw [← this]
+      clear this
+      rfl
+    · rw [Turn_not_fst_iff_snd, Turn_snd_fst_step] at q
+      rw [if_pos q]
+      dsimp [history_on_turn]
+      rw [← Turn_fst_step, Turn_fst_not_step] at q
+      rw [if_neg q]
+      rw [fst_strat_deconditioned, if_neg (by apply History_on_turn_nonempty_of_succ)]
+      have := g.History_of_deconditioned fst_act f_strat s_strat t
+      dsimp at this
+      rw [this]
+      rw [List.dropLast_concat]
+      rw [← this]
+      clear this
+      have := tb.1 f_strat s_strat fst_act fst_act_legal
+      dsimp at this
+      specialize this t (s_strat (world_after_fst g fst_act).init_game_state (History_on_turn (Symm_Game_World.transition g g.init_game_state [] fst_act) f_strat s_strat t))
+      rw [← Symm_Game_World.world_after_fst_init] at this
+      rw [← Symm_Game_World.world_after_fst_init]
+      rw [← this]
+
+
+lemma zSymm_Game_World.State_of_deconditioned
+  (g: zSymm_Game_World α β)
+  (fst_act: β)
+  (fst_act_legal: g.law g.init_game_state [] fst_act)
+  (f_strat s_strat : Strategy α β)
+  (turn : ℕ):
+  let fst_strat := fst_strat_deconditioned s_strat fst_act g.toSymm_Game_World
+  let snd_strat := snd_strat_deconditioned f_strat fst_act g.toSymm_Game_World
+  g.state_on_turn fst_strat snd_strat (turn + 1) =
+  (g.world_after_fst fst_act).state_on_turn f_strat s_strat turn :=
+  by
+  apply Symm_Game_World.State_of_deconditioned
+  · apply Symm_Game_World.strong_transition_blind_toWeak
+    apply Symm_Game_World.hyper_transition_blind_toStrong
+    apply zSymm_Game_World.is_hyper_transition_blind
+  · exact fst_act_legal
+
+
+
+
+lemma Symm_Game_World.law_deconditioned_fst
+  (g: Symm_Game_World α β)
+  (fst_act: β)
+  (fst_act_legal: g.law g.init_game_state [] fst_act)
+  (f_strat s_strat : Strategy α β)
+  (s_leg: Strategy_legal_snd (g.world_after_fst fst_act).init_game_state (g.world_after_fst fst_act).law f_strat s_strat)
+  (b : g.legal_blind_fst)
+  :
+  let fst_strat := fst_strat_deconditioned s_strat fst_act g
+  let snd_strat := snd_strat_deconditioned f_strat fst_act g
+  Strategy_legal_fst g.init_game_state g.law fst_strat snd_strat :=
+  by
+  intro fst_strat snd_strat t tf
+  cases' t with t
+  · dsimp [History_on_turn, fst_strat_deconditioned]
+    rw [if_pos (by rfl)]
+    exact fst_act_legal
+  · rw [← b, Symm_Game_World.History_of_deconditioned]
+    · dsimp [History_on_turn, fst_strat_deconditioned]
+      rw [if_neg (by apply List.append_ne_nil_of_ne_nil_right ; exact List.cons_ne_nil fst_act [])]
+      rw [List.dropLast_concat]
+      apply s_leg
+      rw [Turn_snd_fst_step]
+      exact tf
+    · exact fst_act_legal
+
+
+lemma Symm_Game_World.law_deconditioned_snd
+  (g: Symm_Game_World α β)
+  (fst_act: β)
+  (fst_act_legal: g.law g.init_game_state [] fst_act)
+  (f_strat s_strat : Strategy α β)
+  (f_leg: Strategy_legal_fst (g.world_after_fst fst_act).init_game_state (g.world_after_fst fst_act).law f_strat s_strat)
+  (b : g.legal_blind_snd)
+  :
+  let fst_strat := fst_strat_deconditioned s_strat fst_act g
+  let snd_strat := snd_strat_deconditioned f_strat fst_act g
+  Strategy_legal_snd g.init_game_state g.law fst_strat snd_strat :=
+  by
+  intro fst_strat snd_strat t tf
+  cases' t with t
+  · contradiction
+  · rw [← b, Symm_Game_World.History_of_deconditioned]
+    · dsimp [History_on_turn, snd_strat_deconditioned]
+      rw [List.dropLast_concat]
+      apply f_leg
+      rw [Turn_fst_snd_step]
+      exact tf
+    · exact fst_act_legal
+
+
+#exit
+
+-- # Blind transition
+
 def Symm_Game_World.transition_blind_fst (g : Symm_Game_World α β) : Prop :=
-  ∀ f_strat s_strat: Strategy α β, ∀ fst_act : β, g.law g.init_game_state [] fst_act →
+  ∀ (f_strat: sStrategy g.init_game_state g.law g.law), ∀ (s_strat: sStrategy g.init_game_state g.law g.law), ∀ fst_act : β, g.law g.init_game_state [] fst_act →
   let fst_strat := fst_strat_deconditioned s_strat fst_act g
   let snd_strat := snd_strat_deconditioned f_strat fst_act g
   ∀ turn : ℕ, ∀ act : β, g.transition (g.world_after_fst fst_act).init_game_state (History_on_turn (g.world_after_fst fst_act).init_game_state f_strat s_strat turn) act
     = g.transition g.init_game_state (History_on_turn g.init_game_state fst_strat snd_strat (turn + 1)) act
 
+#exit
 def Symm_Game_World.transition_blind_snd (g : Symm_Game_World α β) : Prop :=
   ∀ f_strat s_strat: Strategy α β, ∀ fst_act : β, g.law g.init_game_state [] fst_act →
   let fst_strat := fst_strat_deconditioned s_strat fst_act g
@@ -171,6 +318,7 @@ def Symm_Game_World.transition_blind_snd (g : Symm_Game_World α β) : Prop :=
   ∀ turn : ℕ, ∀ act : β, g.transition (g.world_after_fst fst_act).init_game_state (History_on_turn (g.world_after_fst fst_act).init_game_state f_strat s_strat turn) act
     = g.transition g.init_game_state (History_on_turn g.init_game_state fst_strat snd_strat (turn + 1)) act
 
+#exit
 
 def Symm_Game_World.transition_blind (g : Symm_Game_World α β) : Prop :=
  g.transition_blind_fst ∧ g.transition_blind_snd
@@ -302,220 +450,8 @@ lemma zSymm_Game_World.is_hyper_transition_blind (g : zSymm_Game_World α β) :
         · exact preh_leg
 
 
-
-
-lemma Symm_Game_World.State_of_deconditioned
-  (g: Symm_Game_World α β)
-  (tb : g.transition_blind)
-  (fst_act: β)
-  (fst_act_legal: g.law g.init_game_state [] fst_act)
-  (f_strat s_strat : Strategy α β)
-  (turn : ℕ):
-  let fst_strat := fst_strat_deconditioned s_strat fst_act g
-  let snd_strat := snd_strat_deconditioned f_strat fst_act g
-  g.state_on_turn fst_strat snd_strat (turn + 1) =
-  (g.world_after_fst fst_act).state_on_turn f_strat s_strat turn :=
-  by
-  intro fst_strat snd_strat
-  cases' turn with t
-  · dsimp [state_on_turn]
-    rw [if_pos (by decide)]
-    dsimp [history_on_turn, History_on_turn]
-    rw [fst_strat_deconditioned, if_pos (by rfl)]
-  · dsimp [state_on_turn]
-    by_cases q : Turn_fst (t + 1)
-    · rw [if_pos q]
-      rw [Turn_fst_not_step] at q
-      rw [if_neg q]
-      dsimp [history_on_turn]
-      have := g.History_of_deconditioned fst_act f_strat s_strat t
-      dsimp at this
-      rw [this]
-      rw [snd_strat_deconditioned, List.dropLast_concat]
-      rw [← this]
-      clear this
-      have := tb.2 f_strat s_strat fst_act fst_act_legal
-      dsimp at this
-      specialize this t (f_strat (world_after_fst g fst_act).init_game_state (History_on_turn (world_after_fst g fst_act).init_game_state f_strat s_strat t))
-      rw [← Symm_Game_World.world_after_fst_init]
-      rw [← this]
-      clear this
-      rfl
-    · rw [Turn_not_fst_iff_snd, Turn_snd_fst_step] at q
-      rw [if_pos q]
-      dsimp [history_on_turn]
-      rw [← Turn_fst_step, Turn_fst_not_step] at q
-      rw [if_neg q]
-      rw [fst_strat_deconditioned, if_neg (by apply History_on_turn_nonempty_of_succ)]
-      have := g.History_of_deconditioned fst_act f_strat s_strat t
-      dsimp at this
-      rw [this]
-      rw [List.dropLast_concat]
-      rw [← this]
-      clear this
-      have := tb.1 f_strat s_strat fst_act fst_act_legal
-      dsimp at this
-      specialize this t (s_strat (world_after_fst g fst_act).init_game_state (History_on_turn (Symm_Game_World.transition g g.init_game_state [] fst_act) f_strat s_strat t))
-      rw [← Symm_Game_World.world_after_fst_init] at this
-      rw [← Symm_Game_World.world_after_fst_init]
-      rw [← this]
-
-
-lemma zSymm_Game_World.State_of_deconditioned
-  (g: zSymm_Game_World α β)
-  (fst_act: β)
-  (fst_act_legal: g.law g.init_game_state [] fst_act)
-  (f_strat s_strat : Strategy α β)
-  (turn : ℕ):
-  let fst_strat := fst_strat_deconditioned s_strat fst_act g.toSymm_Game_World
-  let snd_strat := snd_strat_deconditioned f_strat fst_act g.toSymm_Game_World
-  g.state_on_turn fst_strat snd_strat (turn + 1) =
-  (g.world_after_fst fst_act).state_on_turn f_strat s_strat turn :=
-  by
-  apply Symm_Game_World.State_of_deconditioned
-  · apply Symm_Game_World.strong_transition_blind_toWeak
-    apply Symm_Game_World.hyper_transition_blind_toStrong
-    apply zSymm_Game_World.is_hyper_transition_blind
-  · exact fst_act_legal
-
-
-
-
-
-
-
--- -- # Careless strat
-
-
--- def Game_World.Strategy_blind_fst (strat : Strategy α β) (g : Game_World α β) : Prop :=
---   ∀ s_strat: Strategy α β,
---   let fst_act := strat g.init_game_state []
---   ∀ turn : ℕ, strat (g.world_after_fst fst_act).init_game_state (History_on_turn (g.world_after_fst fst_act).init_game_state s_strat strat turn)
---     = strat g.init_game_state (History_on_turn g.init_game_state strat s_strat (turn + 1))
-
-
--- def Game_World.Strategy_blind_snd (strat : Strategy α β) (g : Game_World α β) : Prop :=
---   ∀ f_strat: Strategy α β,
---   let fst_act := f_strat g.init_game_state []
---   ∀ turn : ℕ, strat (g.world_after_fst fst_act).init_game_state (History_on_turn (g.world_after_fst fst_act).init_game_state strat f_strat turn)
---     = strat g.init_game_state (History_on_turn g.init_game_state f_strat strat (turn + 1))
-
--- def Game_World.Strategy_blind (strat : Strategy α β) (g : Game_World α β) : Prop :=
---   g.Strategy_blind_fst strat ∧ g.Strategy_blind_snd strat
-
--- def Game_World.strong_Strategy_blind (strat : Strategy α β) (g : Game_World α β) : Prop :=
---   ∀ fst_act : β, g.law g.init_game_state [] fst_act →
---   ∀ hist : List β, strat (g.world_after_fst fst_act).init_game_state hist
---     = strat g.init_game_state (hist ++ [fst_act])
-
--- lemma Game_World.world_after_fst_History_blind (g : Game_World α β)
---   (f_strat s_strat : Strategy α β) (turn : ℕ)
---   (hf : g.Strategy_blind_fst f_strat) (hs : g.Strategy_blind_snd s_strat)
---   :
---   (History_on_turn (g.world_after_fst (f_strat g.init_game_state [])).init_game_state s_strat f_strat turn)
---   ++ [(f_strat g.init_game_state [])] = History_on_turn g.init_game_state f_strat s_strat (turn+1) :=
---   by
---   rw [History_on_turn]
---   induction' turn with t ih
---   · dsimp [History_on_turn]
---     rw [if_pos (by decide)]
---   · dsimp [History_on_turn]
---     by_cases q : Turn_fst (t+1)
---     · rw [if_pos q] at *
---       rw [Turn_fst_not_step] at q
---       rw [if_neg q]
---       rw [← Turn_fst_not_step] at q
---       rw [if_pos q]
---       rw [Game_World.world_after_fst_init] at *
---       rw [List.cons_append, ih]
---       congr 1
---       have := hs f_strat t
---       rw [← Game_World.world_after_fst_init, this]
---       dsimp [History_on_turn]
---       rw [if_pos q]
---     · rw [if_neg q] at *
---       rw [Turn_fst_not_step, not_not] at q
---       rw [if_pos q]
---       rw [← @not_not (Turn_fst (t + 1 + 1)), ← Turn_fst_not_step] at q
---       rw [if_neg q]
---       rw [Game_World.world_after_fst_init] at *
---       rw [List.cons_append]
---       congr 1
---       have := hf s_strat t
---       rw [Game_World.world_after_fst_init] at this
---       rw [this]
---       dsimp [History_on_turn]
---       rw [if_neg q]
-
-
--- lemma Game_World.world_after_fst_History_strong_blind (g : Game_World α β)
---   (f_strat s_strat : Strategy α β) (turn : ℕ)
---   (f_leg : Strategy_legal_fst g.init_game_state g.law f_strat s_strat)
---   (hf : g.strong_Strategy_blind f_strat) (hs : g.strong_Strategy_blind s_strat)
---   :
---   (History_on_turn (g.world_after_fst (f_strat g.init_game_state [])).init_game_state s_strat f_strat turn)
---   ++ [(f_strat g.init_game_state [])] = History_on_turn g.init_game_state f_strat s_strat (turn+1) :=
---   by
---   rw [History_on_turn]
---   induction' turn with t ih
---   · dsimp [History_on_turn]
---     rw [if_pos (by decide)]
---   · unfold History_on_turn
---     by_cases q : Turn_fst (t+1)
---     · rw [if_pos q]
---       rw [List.cons_append, ih]
---       specialize hs (f_strat g.init_game_state []) (by apply f_leg 0 (by decide)) (History_on_turn (Game_World.transition g g.init_game_state [] (f_strat g.init_game_state [])) s_strat f_strat t)
---       rw [← Game_World.world_after_fst_init] at hs
---       rw [hs, ih]
---       rw [if_neg (show ¬ Turn_fst (Nat.succ t + 1) from (by rw [← Turn_fst_not_step]; exact q))]
---     · rw [if_neg q]
---       rw [List.cons_append, ih]
---       specialize hf (f_strat g.init_game_state []) (by apply f_leg 0 (by decide)) (History_on_turn (Game_World.transition g g.init_game_state [] (f_strat g.init_game_state [])) s_strat f_strat t)
---       rw [← Game_World.world_after_fst_init] at hf
---       rw [hf, ih]
---       rw [if_pos (show Turn_fst (Nat.succ t + 1) from (by rw [iff_not_comm.mp (Turn_fst_not_step (t+1))]; exact q))]
-
-
--- -- might not be the case, because we have no carelessness of other strat
--- -- lemma Game_World.strong_Strategy_blind_toWeak (strat : Strategy α β) (g : Game_World α β)
--- --   (f_leg : Strategy_legal_fst g.init_game_state g.law strat s_strat) :
--- --   g.strong_Strategy_blind strat → g.Strategy_blind strat :=
--- --   by
--- --   intro hyp
--- --   constructor
--- --   · intro s_strat f_act t
--- --     rw [hyp]
-
-
-
--- --#exit
-
--- def Game_World.hyper_Strategy_blind
---   (strat : Strategy α β) (g : Game_World α β) : Prop :=
---   ∀ prehist : List β, Hist_legal g.law g.law g.init_game_state prehist →
---   ∀ hist : List β, strat (g.world_after_preHist prehist).init_game_state hist
---     = strat g.init_game_state (hist ++ prehist)
-
-
--- lemma Game_World.hyper_Strategy_blind_toStrong
---   (strat : Strategy α β) (g : Game_World α β) :
---   g.hyper_Strategy_blind strat → g.strong_Strategy_blind strat :=
---   by
---   intro hyp
---   intro f_act f_leg hist
---   specialize hyp [f_act] _ hist
---   · apply Hist_legal.cons
---     · dsimp
---       rw [if_pos (by decide)]
---       exact f_leg
---     · apply Hist_legal.nil
---   · dsimp [Game_World.world_after_fst, Game_World.world_after_preHist] at *
---     exact hyp
-
-
---#exit
-
 -- # Blind law
+
 
 def Symm_Game_World.legal_blind_fst (g : Symm_Game_World α β) : Prop :=
   ∀ f_strat s_strat: Strategy α β, ∀ fst_act : β, g.law g.init_game_state [] fst_act →
@@ -645,55 +581,9 @@ lemma zSymm_Game_World.is_hyper_legal_blind (g : zSymm_Game_World α β) :
         · exact preh_leg
 
 
-lemma Symm_Game_World.law_deconditioned_fst
-  (g: Symm_Game_World α β)
-  (fst_act: β)
-  (fst_act_legal: g.law g.init_game_state [] fst_act)
-  (f_strat s_strat : Strategy α β)
-  (s_leg: Strategy_legal_snd (g.world_after_fst fst_act).init_game_state (g.world_after_fst fst_act).law f_strat s_strat)
-  (b : g.legal_blind_fst)
-  :
-  let fst_strat := fst_strat_deconditioned s_strat fst_act g
-  let snd_strat := snd_strat_deconditioned f_strat fst_act g
-  Strategy_legal_fst g.init_game_state g.law fst_strat snd_strat :=
-  by
-  intro fst_strat snd_strat t tf
-  cases' t with t
-  · dsimp [History_on_turn, fst_strat_deconditioned]
-    rw [if_pos (by rfl)]
-    exact fst_act_legal
-  · rw [← b, Symm_Game_World.History_of_deconditioned]
-    · dsimp [History_on_turn, fst_strat_deconditioned]
-      rw [if_neg (by apply List.append_ne_nil_of_ne_nil_right ; exact List.cons_ne_nil fst_act [])]
-      rw [List.dropLast_concat]
-      apply s_leg
-      rw [Turn_snd_fst_step]
-      exact tf
-    · exact fst_act_legal
+#exit
 
 
-lemma Symm_Game_World.law_deconditioned_snd
-  (g: Symm_Game_World α β)
-  (fst_act: β)
-  (fst_act_legal: g.law g.init_game_state [] fst_act)
-  (f_strat s_strat : Strategy α β)
-  (f_leg: Strategy_legal_fst (g.world_after_fst fst_act).init_game_state (g.world_after_fst fst_act).law f_strat s_strat)
-  (b : g.legal_blind_snd)
-  :
-  let fst_strat := fst_strat_deconditioned s_strat fst_act g
-  let snd_strat := snd_strat_deconditioned f_strat fst_act g
-  Strategy_legal_snd g.init_game_state g.law fst_strat snd_strat :=
-  by
-  intro fst_strat snd_strat t tf
-  cases' t with t
-  · contradiction
-  · rw [← b, Symm_Game_World.History_of_deconditioned]
-    · dsimp [History_on_turn, snd_strat_deconditioned]
-      rw [List.dropLast_concat]
-      apply f_leg
-      rw [Turn_fst_snd_step]
-      exact tf
-    · exact fst_act_legal
 
 
 
